wip

src/lib/Entity/Map.ml
@@ -1,0 +1,3 @@
+type t = Kernel.t1
+
+let all_wall_map = Kernel.all_wall_map
