src/lib/Entity/Map.mli
@@ -1,0 +1,3 @@
+type t = Kernel.t1
+
+val all_wall_map : Big_int_Z.big_int -> Big_int_Z.big_int -> t
