src/lib/Coquill/Array.v
@@ -1,1 +1,24 @@
 Set Default Goal Selector "!". 
+
+From Coq Require Import NArith.
+From Coquill Require Import List.
+
+Open Scope N_scope.
+
+Create HintDb array.
+
+Record t (A : Type) (n : N) : Type := make {
+  inner_list : list A;
+  length_spec : length inner_list = n;
+}.
+
+Hint Constructors t : array.
+
+Definition empty (A : Type) : t A 0 := make A 0 [] eq_refl.
+
+Program Definition repeat {A : Type} (x : A) (n : N) : t A n :=
+  make A n (List.repeat x n) _.
+Next Obligation.
+Proof.
+  apply repeat_length.
+Qed.
