src/lib/Coquill/NonEmptyArray.v
@@ -1,0 +1,12 @@
+Set Default Goal Selector "!".
+
+From Coquill Require Array.
+From Coquill Require Import List.
+From Coquill Require Import PArith.
+
+Definition t (A : Type) (n : positive) : Type := Array.t A (Npos n).
+
+Definition make {A : Type} (n : positive) (data : Array.t A (Npos n)) : t A n := data.
+
+Program Definition repeat {A : Type} (x : A) (n : positive) : t A n :=
+  make n (Array.repeat x (Npos n)).
