src/lib/Kernel/Map.v
@@ -1,0 +1,13 @@
+Set Default Goal Selector "!".
+
+From Coq Require Import ZArith.
+From Coq Require Import Lia.
+From Coquill Require NonEmptyArray.
+From Coquill Require Import PArith.
+
+Open Scope Z_scope.
+
+Definition t (width height : positive) : Type := NonEmptyArray.t (NonEmptyArray.t bool width) height.
+
+Definition all_wall_map (width height : positive) : t width height :=
+  NonEmptyArray.repeat (NonEmptyArray.repeat true width) height.
